cava/Cava/Acorn/Multistep.v
@@ -1,0 +1,81 @@
+(****************************************************************************)
+(* Copyright 2021 The Project Oak Authors                                   *)
+(*                                                                          *)
+(* Licensed under the Apache License, Version 2.0 (the "License")           *)
+(* you may not use this file except in compliance with the License.         *)
+(* You may obtain a copy of the License at                                  *)
+(*                                                                          *)
+(*     http://www.apache.org/licenses/LICENSE-2.0                           *)
+(*                                                                          *)
+(* Unless required by applicable law or agreed to in writing, software      *)
+(* distributed under the License is distributed on an "AS IS" BASIS,        *)
+(* WITHOUT WARRANTIES OR CONDITIONS OF ANY KIND, either express or implied. *)
+(* See the License for the specific language governing permissions and      *)
+(* limitations under the License.                                           *)
+(****************************************************************************)
+
+Require Import Coq.Lists.List.
+Import ListNotations.
+
+Require Import Cava.ListUtils.
+Require Import Cava.Tactics.
+Require Import Cava.Acorn.CavaClass.
+Require Import Cava.Acorn.Circuit.
+Require Import Cava.Acorn.Combinational.
+Require Import Cava.Acorn.IdentityNew.
+
+(* Run a circuit for many timesteps, starting at the reset value *)
+Definition multistep {i o} (c : Circuit i o) (input : list i) : list o :=
+  match input with
+  | [] => []
+  | i :: input =>
+    let '(o,st) := unIdent (interp c (reset_state c) i) in
+    let '(acc, _) := fold_left_accumulate
+                       (fun o_st i => unIdent (interp c (snd o_st) i))
+                       input (o,st) in
+    map fst acc
+  end.
+
+Lemma multistep_compose {A B C} (c1 : Circuit A B) (c2 : Circuit B C) (input : list A) :
+  multistep (Compose c1 c2) input = multistep c2 (multistep c1 input).
+Proof.
+  clear.
+  cbv [multistep]. destruct input as [|i0 input]; [ reflexivity | ].
+  repeat destruct_pair_let; simpl_ident.
+  destruct input as [|i1 input]; [ cbn; repeat destruct_pair_let; reflexivity | ].
+  rewrite !fold_left_accumulate_cons_full.
+  cbn [fst snd map interp reset_state circuit_state].
+  repeat first [ destruct_pair_let | progress simpl_ident ].
+  rewrite <-!surjective_pairing.
+  rewrite fold_left_accumulate_map.
+  rewrite fold_left_accumulate_fold_left_accumulate.
+  cbn [map]. apply f_equal.
+  factor_out_loops.
+  eapply fold_left_accumulate_double_invariant
+    with (I:=fun (x : B * circuit_state c1 * (C * circuit_state c2))
+               (y : C * (circuit_state c1 * circuit_state c2)) =>
+               y = (fst (snd x), (snd (fst x), snd (snd x)))).
+  { reflexivity. }
+  { intros. repeat first [ destruct_pair_let | progress simpl_ident ].
+    subst. cbn [fst snd]. reflexivity. }
+  { intros b d acc1 acc2; intros ? Hnth. cbn [fst snd].
+    assert (length acc1 = length acc2) by length_hammer.
+    rewrite <-Forall2_nth_iff in Hnth by length_hammer.
+    apply list_eq_elementwise; [ symmetry; length_hammer | ].
+    intros. autorewrite with push_length in *. rewrite map_map.
+    rewrite map_nth_inbounds with (d2:=d) by length_hammer.
+    erewrite map_nth_inbounds with (d2:=b) by length_hammer.
+    erewrite Hnth by Lia.lia. cbn [fst snd]. reflexivity. }
+Qed.
+
+Lemma multistep_comb {A B} (c : A -> ident B) (input : list A) :
+  multistep (Comb c) input = map (fun a => unIdent (c a)) input.
+Proof.
+  clear.
+  cbv [multistep]. destruct input as [|i0 input]; [ reflexivity | ].
+  repeat destruct_pair_let; simpl_ident.
+  cbn [fst snd map interp reset_state circuit_state].
+  simpl_ident. rewrite fold_left_accumulate_to_map.
+  cbn [map fst]. rewrite map_map. cbn [fst].
+  reflexivity.
+Qed.
